Prove the finite nature of heaps a much easier way

Heap.v
@@ -1,11 +1,12 @@
 Require Import
   Fiat.ADT
   Fiat.ADTNotation
+  Here.TupleEnsembles
+  Coq.Sets.Finite_sets
+  Coq.Sets.Finite_sets_facts
   Here.Nomega
   Here.Decidable
   Here.BindDep
-  Here.FunRelation
-  Here.FinRelation
   Here.Tactics
   Here.ADTInduction.
 
@@ -29,7 +30,7 @@ Variable Zero  : Word8.
 
 Record MemoryBlock := {
   memSize : N;
-  memData : FunRel N Word8
+  memData : Ensemble (N * Word8)
 }.
 
 Ltac tsubst :=
@@ -45,205 +46,70 @@ Ltac tsubst :=
     end;
   subst.
 
-Record CorrectMemoryBlock (blk : MemoryBlock) : Prop := {
-  _ : 0 < memSize blk;
-  _ : forall off, Member off (memData blk) -> off < memSize blk
-}.
-
-Definition Heap := FunRel N MemoryBlock.
-
-Definition CorrectHeap (mem : Heap) :=
-  All (fun p => CorrectMemoryBlock (snd p)) mem.
-
-Ltac against_definition function len tac :=
-  unfold CorrectHeap, All, function; intros;
-  try destruct len; simpl in *;
-  simplify_ensembles; simpl in *; decisions; tsubst;
-  simplify_ensembles; simpl in *; decisions; tsubst; firstorder;
-  intros; decisions; tsubst;
-  tac; decisions; try nomega; firstorder.
-
-Definition shift_address (addr1 addr2 : N) : Heap -> Heap := Move addr1 addr2.
-
-Lemma shift_address_correct `(_ : CorrectHeap mem) :
-  forall addr1 addr2, CorrectHeap (shift_address addr1 addr2 mem).
-Proof.
-  against_definition shift_address len idtac.
-Qed.
-
-Definition fit_to_length (addr : N) (len : N | 0 < len) : Heap -> Heap :=
-  Modify addr (fun blk =>
-                 {| memSize := ` len
-                  ; memData := Filter (fun p => fst p < ` len)
-                                      (memData blk) |}).
-
-Lemma fit_to_length_correct `(_ : CorrectHeap mem) :
-  forall addr len, CorrectHeap (fit_to_length addr len mem).
-Proof.
-  against_definition fit_to_length len idtac.
-Qed.
-
-Definition set_address (addr : N) (w : Word8) : Heap -> Heap :=
-  Map (fun p =>
-         let (base, blk) := p in
-         IfDec within base (memSize blk) addr
-         Then {| memSize := memSize blk
-               ; memData := Update (addr - base) w (memData blk) |}
-         Else blk).
-
-Lemma set_address_correct `(_ : CorrectHeap mem) :
-  forall addr w, CorrectHeap (set_address addr w mem).
-Proof.
-  against_definition set_address len simplify_ensembles.
-Qed.
-
-Definition copy_memory
-        (addr1 addr2 : N) (len : N) (mem : Heap) : Comp (Heap * unit) :=
-  ms <- { ms : option (N * MemoryBlock)
-        | forall addr' blk', ms = Some (addr', blk') ->
-            0 < len /\ Find (fun addr' blk' =>
-                               fits addr' (memSize blk') addr1 len)
-                            addr' blk' mem };
-  md <- { md : option (N * MemoryBlock)
-        | forall addr' blk', md = Some (addr', blk') ->
-            0 < len /\ Find (fun addr' blk' =>
-                               fits addr' (memSize blk') addr2 len)
-                            addr' blk' mem };
-  ret (match ms, md with
-       | Some (saddr, sblk), Some (daddr, dblk) =>
-         Update daddr {| memSize := memSize dblk
-                       ; memData :=
-                           let soff := addr1 - saddr in
-                           let doff := addr2 - daddr in
-                           Overlay (fun a =>
-                                      IfDec within doff len a
-                                      Then Some (soff + (a - doff))
-                                      Else None)
-                                   (memData dblk) (memData sblk) |} mem
-       | _, _ => mem
-       end, tt).
-
-Lemma copy_memory_correct `(_ : CorrectHeap mem) :
-  forall addr1 addr2 len mem',
-    copy_memory addr1 addr2 len mem ↝ (mem', tt) -> CorrectHeap mem'.
-Proof.
-  unfold CorrectHeap, All, copy_memory; intros.
-  simplify_ensembles; simpl in *.
-  destruct x, x0;
-  simplify_ensembles; simpl in *; decisions; tsubst.
-  - inv H0.
-      firstorder.
-    inv H2.
-    rename n1 into saddr.
-    rename m1 into sblk.
-    rename n into daddr.
-    rename m0 into dblk.
-    destruct (H saddr sblk eq_refl); clear H.
-    destruct (H1 daddr dblk eq_refl); clear H1 H0.
-    destruct H2, H3.
-    destruct (CorrectHeap0 _ H0).
-    destruct (CorrectHeap0 _ H2).
-    simpl in *.
-    constructor; auto; simpl; intros.
-    destruct H8.
-    unfold Overlay, Ensembles.In in *; simpl in *.
-    specialize (H8 (addr1 - saddr + (off - (addr2 - daddr)))).
-    decisions.
-    + destruct H8; teardown; intuition.
-      unfold Member in *.
-      specialize (H5 (addr1 - saddr + (off - (addr2 - daddr)))).
-      assert (exists b : Word8,
-                 In (N * Word8) (relEns (memData sblk))
-                    (addr1 - saddr + (off - (addr2 - daddr)), b)).
-        exists x.
-        assumption.
-      specialize (H5 H10).
-      unfold fits in *.
-      teardown.
-      unfold within in *.
-      clear -H1 H12 H H3 H11 H4 H5 H6 Heqe.
-      nomega.
-    + destruct H8; teardown.
-        discriminate.
-      firstorder.
-  - firstorder.
-  - firstorder.
-  - firstorder.
-Qed.
-
-Definition set_memory (addr : N) (len : N) (w : Word8) :
-  Heap -> Heap :=
-  Map (fun p =>
-         let (base, blk) := p in
-         IfDec fits base (memSize blk) addr len
-         Then {| memSize := memSize blk
-               ; memData := Define (within (addr - base) len) w
-                                   (memData blk) |}
-         Else blk).
-
-Lemma set_memory_correct `(_ : CorrectHeap mem) :
-  forall addr len w, CorrectHeap (set_memory addr len w mem).
-Proof.
-  against_definition set_memory len ltac:(unfold Ensembles.In in *; simpl in *).
-Qed.
-
-Definition free_block (addr : N) : Heap -> Heap := Remove addr.
-
-Lemma free_block_correct `(_ : CorrectHeap mem) :
-  forall addr, CorrectHeap (free_block addr mem).
-Proof.
-  against_definition free_block len idtac.
-Qed.
-
-Definition find_free_block (len : N | 0 < len) (mem : Heap) : Comp N :=
-  { addr : N | forall addr' blk',
-      ~ Find (fun addr' blk' =>
-                overlaps addr' (memSize blk') addr (` len))
-             addr' blk' mem }.
-
-Lemma find_free_block_spec (len : N | 0 < len) `(_ : CorrectHeap r) :
-  forall addr, find_free_block len r ↝ addr -> ~ Member addr r.
-Proof.
-  simplify_ensembles.
-  unfold not; intros.
-  apply Member_Lookup in H0; destruct H0.
-  specialize (H addr x).
-  apply (LogicFacts.not_and_implication (Lookup _ _ _)) in H; eauto.
-  destruct (All_Lookup _ _ _ r CorrectHeap0 _ _ H0).
-  contradiction (overlaps_irr addr H1 (proj2_sig len)).
-Qed.
+Ltac inspect :=
+  repeat (
+    teardown; tsubst; simpl in *; decisions;
+    try match goal with
+      | [ H1 : ~ overlaps ?X ?Y ?X ?Z,
+          H2 : 0 < ?Y,
+          H3 : 0 < ?Z |- _ ] => pose proof (overlaps_irr X H2 H3); contradiction
+      | [ H : ~ overlaps ?X ?Y ?A ?B |- ~ overlaps ?A ?B ?X ?Y ] =>
+        let H0 := fresh "H0" in
+        unfold not; intro H0; apply overlaps_sym in H0; contradiction
+    end).
 
 Definition HeapSpec := Def ADT {
   (* a mapping of addr tokens to a length, and another mapping from
      offsets within a certain block to individual bytes *)
-  rep := Heap,
+  rep := Ensemble (N * MemoryBlock),
 
-  Def Constructor0 emptyS : rep := ret (Empty _ _),,
+  Def Constructor0 emptyS : rep := ret Empty,,
 
   (* Allocation returns the address for the newly allocated block. Note that
      conditions such as out-of-memory are not handled here; the final
      implementation must decide how to handle this operationally, such as
      throwing an exception. *)
   Def Method1 allocS (r : rep) (len : N | 0 < len) : rep * N :=
-    addr <- find_free_block len r;
+    addr <- { addr : N
+            | All (fun addr' blk' =>
+                     ~ overlaps addr' (memSize blk') addr (` len)) r };
     ret (Update addr {| memSize := ` len
-                      ; memData := Empty _ _ |} r, addr),
+                      ; memData := Empty |} r, addr),
 
   (* Freeing an unallocated block is a no-op. *)
   Def Method1 freeS (r : rep) (addr : N) : rep * unit :=
-    ret (free_block addr r, tt),
+    ret (Remove addr r, tt),
 
   (* Realloc is not required to reuse the same block. If the address does not
      identify an allociated region, a new memory block is returned without any
      bytes moved. *)
   Def Method2 reallocS (r : rep) (addr : N) (len : N | 0 < len) : rep * N :=
-    b <- { b : bool | forall blk, decides b (Lookup addr blk r) };
-    naddr <- find_free_block len (free_block addr r);
-    ret (If b
-         Then fit_to_length naddr len (shift_address addr naddr r)
-         Else Update naddr {| memSize := ` len
-                            ; memData := Empty _ _ |} r,
-         naddr),
+    present <- { blk : option MemoryBlock
+               | Ifopt blk as blk'
+                 Then Lookup addr blk' r
+                 Else ~ Member addr r };
+    naddr   <- { naddr : N
+               | All (fun addr' blk' =>
+                        ~ overlaps addr' (memSize blk') naddr (` len))
+                     (Remove addr r) };
+    ret (
+      Ifopt present as blk
+      Then IfDec naddr = addr
+           Then Modify addr
+                  (fun blk =>
+                     {| memSize := ` len
+                      ; memData := IfDec memSize blk < ` len
+                                   Then memData blk
+                                   Else Filter (fun pos _ => pos < ` len)
+                                               (memData blk) |}) r
+           Else Update naddr (IfDec memSize blk < ` len
+                              Then blk
+                              Else (* No copy is done because it does not fit *)
+                                   {| memSize := ` len
+                                    ; memData := Empty |}) (Remove addr r)
+      Else Update naddr {| memSize := ` len
+                         ; memData := Empty |} r,
+      naddr),
 
   (* Peeking an unallocated address allows any value to be returned. *)
   Def Method1 peekS (r : rep) (addr : N) : rep * Word8 :=
@@ -255,26 +121,57 @@ Definition HeapSpec := Def ADT {
                    position.
                 2. Peeking an allocated, uninitialized byte.
                 3. Peeking at an unallocated location. *)
-             Find (fun a b => within a (memSize b) addr) base blk' r
+             Lookup base blk' r
+               -> within base (memSize blk') addr
                -> forall v, Lookup (addr - base) v (memData blk')
                -> p = v };
     ret (r, p),
 
   (* Poking an unallocated address is a no-op and returns false. *)
   Def Method2 pokeS (r : rep) (addr : N) (w : Word8) : rep * unit :=
-    ret (set_address addr w r, tt),
+    ret (Map (fun base blk =>
+                IfDec within base (memSize blk) addr
+                Then {| memSize := memSize blk
+                      ; memData := Update (addr - base) w (memData blk) |}
+                Else blk) r, tt),
 
   (* Data may only be copied from one allocated block to another (or within
      the same block), and the region must fit within both source and
      destination. Otherwise, the operation is a no-op and returns false. *)
   Def Method3 memcpyS (r : rep) (addr1 : N) (addr2 : N) (len : N) :
-    rep * unit := copy_memory addr1 addr2 len r,
+    rep * unit :=
+    ms <- { ms : option (N * MemoryBlock)
+          | forall addr' blk', ms = Some (addr', blk') ->
+              0 < len /\ Lookup addr' blk' r /\
+              fits addr' (memSize blk') addr1 len };
+    md <- { md : option (N * MemoryBlock)
+          | forall addr' blk', md = Some (addr', blk') ->
+              0 < len /\ Lookup addr' blk' r /\
+              fits addr' (memSize blk') addr2 len };
+    ret (match ms, md with
+         | Some (saddr, sblk), Some (daddr, dblk) =>
+           Update daddr {| memSize := memSize dblk
+                         ; memData :=
+                             let soff := addr1 - saddr in
+                             let doff := addr2 - daddr in
+                             Overlay (fun a =>
+                                        IfDec within doff len a
+                                        Then Some (soff + (a - doff))
+                                        Else None)
+                                     (memData dblk) (memData sblk) |} r
+         | _, _ => r
+         end, tt),
 
   (* Any attempt to memset bytes outside of an allocated block is a no-op that
      returns false. *)
   Def Method3 memsetS (r : rep) (addr : N) (len : N) (w : Word8) :
     rep * unit :=
-    ret (set_memory addr len w r, tt)
+    ret (Map (fun base blk =>
+                IfDec fits base (memSize blk) addr len
+                Then {| memSize := memSize blk
+                      ; memData := Define (within (addr - base) len) w
+                                          (memData blk) |}
+                Else blk) r, tt)
 
 }%ADTParsing.
 
@@ -308,229 +205,194 @@ Definition memset (r : Rep HeapSpec) (addr : N) (len : N) (w : Word8) :
   Comp (Rep HeapSpec * unit) :=
   Eval simpl in callMeth HeapSpec memsetS r addr len w.
 
-Theorem allocations_are_correct :
-  forall r : Rep HeapSpec, fromADT _ r -> CorrectHeap r.
-Proof.
-  unfold CorrectHeap, All; intros.
-  generalize dependent p.
-  ADT induction r.
-  - constructor; inversion H0.
-  - destruct x; simpl in *.
-    inv H1.
-      inv H2.
-      exact (IHfromADT _ H1).
-    simplify_ensembles.
-    constructor; firstorder.
-  - inv H1; firstorder.
-  - destruct x0; simpl in *.
-    destruct v.
-      exact (fit_to_length_correct (@shift_address_correct _ IHfromADT _ _) H1).
-    inv H1; firstorder.
-      inv H2; trivial.
-    inv H2; inv H1.
-  - exact (set_address_correct IHfromADT H1).
-  - destruct x2.
-    pose proof (copy_memory_correct IHfromADT H0).
-    exact (H2 _ H1).
-  - exact (set_memory_correct IHfromADT H1).
-Qed.
+(**
+ ** Theorems related to the Heap specification.
+ **)
 
-Corollary allocations_have_size : forall r : Rep HeapSpec, fromADT _ r ->
-  forall addr len data,
-    Lookup addr {| memSize := len; memData := data |} r -> 0 < len.
+Ltac complete IHfromADT :=
+  inspect;
+  try match goal with
+    [ H : (?X =? ?Y) = true |- _ ] => apply N.eqb_eq in H; subst
+  end;
+  try (eapply IHfromADT; eassumption);
+  try solve [ eapply IHfromADT; try eassumption; inspect
+            | try eapply IHfromADT; eassumption
+            | inspect;
+              try (unfold fits, within in *; inspect; nomega);
+              eapply IHfromADT; try eassumption; inspect
+            | discriminate ].
+
+Theorem allocations_have_size : forall r : Rep HeapSpec, fromADT _ r ->
+  forall addr blk, Lookup addr blk r -> 0 < memSize blk.
 Proof.
   intros.
-  destruct (allocations_are_correct H _ H0) as [H1 _].
-  exact H1.
+  generalize dependent blk.
+  generalize dependent addr.
+  ADT induction r; [inversion H0|..];
+  complete IHfromADT.
 Qed.
 
-Ltac reveal_no_overlap r :=
+Theorem allocations_correct_offsets : forall r : Rep HeapSpec, fromADT _ r ->
+  forall addr blk, Lookup addr blk r ->
+    forall off, Member off (memData blk) -> off < memSize blk.
+Proof.
+  intros.
+  generalize dependent off.
+  generalize dependent blk.
+  generalize dependent addr.
+  ADT induction r; [inversion H0|..]; inspect;
+  complete IHfromADT.
+  - apply (IHfromADT x) in H2; trivial; nomega.
+Qed.
+
+Ltac match_sizes H IHfromADT :=
   match goal with
-  | [ H1 : forall addr' blk',
-        ~ Find (fun a b => overlaps a (memSize b) ?A1 ?B1) addr' blk' _,
-        H2 : Lookup ?A2 ?B2 _ |- _ ] =>
-    specialize (H1 A2 B2);
-    apply (LogicFacts.not_and_implication (Lookup _ _ _)) in H1; eauto
-  | [ H1 : forall addr' blk',
-        ~ Find (fun a b => overlaps a (memSize b) ?A1 ?B1) addr' blk' _,
-        H2 : Ensembles.In _ _ (?A2, ?B2) |- _ ] =>
-    specialize (H1 A2 B2);
-    apply (LogicFacts.not_and_implication (Lookup _ _ _)) in H1; eauto
+  | [ H1 : Lookup ?A ?X ?R, H2 : Lookup ?B ?Y ?R |- _ ] =>
+    specialize (IHfromADT _ _
+                  H1 (allocations_have_size H _ _ H1) _
+                  H2 (allocations_have_size H _ _ H2)); subst
+  end; inspect; auto.
+
+Ltac match_sizes_r H IHfromADT :=
+  match goal with
+  | [ H1 : Lookup ?A ?X ?R, H2 : Lookup ?B ?Y ?R |- _ ] =>
+    try rewrite <- (IHfromADT _ _
+                      H1 (allocations_have_size H _ _ H1) _
+                      H2 (allocations_have_size H _ _ H2)) in *
+  end; inspect; auto.
+
+Ltac check_overlaps :=
+  match goal with
+    [ H1 : All (fun addr' blk' => ~ overlaps addr' (memSize blk') ?XA ?XL)
+               (Remove ?YA ?R),
+      H2 : ?XA <> ?YA,
+      H3 : 0 < ?XL,
+      H4 : Lookup ?XA ?B ?R,
+      H5 : 0 < memSize ?B |- _ ] =>
+    eapply All_Remove_Lookup_inv with (a':=XA) in H1; eauto;
+    contradiction (overlaps_irr XA H5 H3)
   end.
 
 Theorem allocations_unique : forall r : Rep HeapSpec, fromADT _ r ->
-  forall addr blk1,
-       Lookup addr blk1 r
-    -> forall blk2, Lookup addr blk2 r
-    -> blk1 = blk2.
+  forall addr blk1, Lookup addr blk1 r ->
+  forall blk2, Lookup addr blk2 r -> blk1 = blk2.
 Proof.
   intros.
+  pose proof (allocations_have_size H _ _ H0).
+  pose proof (allocations_have_size H _ _ H1).
   generalize dependent blk2.
   generalize dependent blk1.
   generalize dependent addr.
-  ADT induction r.
-  - inversion H0.
-  - unfold find_free_block in H0.
-    teardown; tsubst; simplify_ensembles.
-    reveal_no_overlap r.
-  - firstorder.
-  - destruct x0; simpl in *.
-    unfold fit_to_length, shift_address in H1, H2.
-    unfold free_block, find_free_block in H0.
-    destruct v; unfold Lookup in *;
-    simplify_ensembles; simpl in *; tsubst; eauto.
-  - unfold set_address in H1, H2.
-    teardown; decisions; tsubst;
-    specialize (IHfromADT _ _ H2 _ H3); subst; eauto;
-    rewrite Heqe in Heqe0; discriminate.
-  - unfold copy_memory in H0.
-    unfold Lookup in *.
-    simplify_ensembles; simpl in *;
-    destruct x3, x4;
-    simplify_ensembles; tsubst;
-    simplify_ensembles;
-    exact (IHfromADT _ _ H1 _ H2).
-  - unfold set_memory in H1, H2.
-    teardown; decisions; tsubst;
-    try destruct x2;
-    try destruct x3;
-    specialize (IHfromADT _ _ H2 _ H3);
-    tsubst; simpl in *; eauto;
-    rewrite Heqe in Heqe0; discriminate.
+  ADT induction r; [inversion H0|..]; inspect;
+  try solve [ match_sizes H IHfromADT ];
+  try discriminate;
+  check_overlaps.
 Qed.
+
+Ltac lookup_uid H :=
+  match goal with
+  | [ H1 : Lookup ?A ?X ?R, H2 : Lookup ?A ?Y ?R |- _ ] =>
+    pose proof (allocations_unique H _ _ H1 _ H2); subst
+  end; inspect; auto.
 
 Corollary allocations_unique_r : forall r : Rep HeapSpec, fromADT _ r ->
-  forall addr1 blk,
-       Lookup addr1 blk r
-    -> forall addr2, ~ Lookup addr2 blk r
-    -> addr1 <> addr2.
+  forall addr1 blk, Lookup addr1 blk r ->
+  forall addr2, ~ Member addr2 r -> addr1 <> addr2.
 Proof.
-  intros.
-  unfold not; intros; subst.
-  ADT induction r.
+  unfold not; intros; subst; ADT induction r;
+  contradiction H1;
+  exists blk;
+  assumption.
 Qed.
 
+Corollary not_overlaps_trans : forall a b x y z,
+  z < y -> ~ overlaps a b x y -> ~ overlaps a b x z.
+Proof. unfold overlaps; intros; nomega. Qed.
+
 Theorem allocations_no_overlap : forall r : Rep HeapSpec, fromADT _ r ->
-  forall addr1 blk1,
-       Lookup addr1 blk1 r
-    -> forall addr2 blk2, Lookup addr2 blk2 r
-    -> addr1 <> addr2
-    -> ~ overlaps addr1 (memSize blk1) addr2 (memSize blk2).
+  forall addr1 blk1, Lookup addr1 blk1 r ->
+  forall addr2 blk2, Lookup addr2 blk2 r
+    -> addr1 <> addr2 -> ~ overlaps addr1 (memSize blk1) addr2 (memSize blk2).
 Proof.
   intros.
+  pose proof (allocations_have_size H _ _ H0).
+  pose proof (allocations_have_size H _ _ H1).
   generalize dependent blk2.
   generalize dependent addr2.
   generalize dependent blk1.
   generalize dependent addr1.
-  ADT induction r.
-  - inversion H0.
-  - unfold find_free_block in H0.
-    teardown; tsubst; simplify_ensembles.
-    + reveal_no_overlap r.
-    + rewrite overlaps_sym.
-      reveal_no_overlap r.
-    + eapply IHfromADT; eassumption.
-  - unfold free_block in H1, H3.
-    teardown; eapply IHfromADT; eassumption.
-  - destruct x0; simpl in *.
-    unfold fit_to_length, shift_address,
-           free_block, find_free_block in *.
-    destruct v; simpl in *;
-    teardown; tsubst; simplify_ensembles; simpl in *.
-    + inv H6. reveal_no_overlap r.
-      apply Lookup_Remove with (a':=x); trivial.
-    + inv H7. reveal_no_overlap r.
-        unfold not; intros.
-        apply overlaps_sym in H7.
-        contradiction.
-      apply Lookup_Remove with (a':=x); trivial.
-    + inv H6; inv H7.
-      eapply IHfromADT; eassumption.
-    + inv H1; inv H3; simplify_ensembles.
-      * eapply IHfromADT; eassumption.
-      * reveal_no_overlap r.
-        apply Lookup_Remove with (a':=x); trivial.
-        eapply allocations_unique_r; eauto.
-      * reveal_no_overlap r.
-          unfold not; intros.
-          apply overlaps_sym in H1.
-          contradiction.
-        apply Lookup_Remove with (a':=x); trivial.
-        eapply allocations_unique_r; eauto.
-  - unfold set_address in H1, H3.
-    teardown; decisions; tsubst; simpl;
-    eapply IHfromADT; eassumption.
-  - unfold copy_memory in H0.
-    unfold Lookup in *.
-    simplify_ensembles; simpl in *.
-    destruct x3, x4;
-    try destruct p;
-    try destruct p0;
-    try specialize (H0 n m eq_refl);
-    try specialize (H4 n0 m0 eq_refl);
-    simplify_ensembles; tsubst;
-    simplify_ensembles;
-    try destruct H6;
-    try destruct H7;
-    eapply IHfromADT; try eassumption.
-  - unfold set_memory in H1, H3.
-    teardown; decisions; tsubst; simpl;
-    eapply IHfromADT; eassumption.
+  ADT induction r; [inversion H0|..];
+  complete IHfromADT;
+  try lookup_uid H;
+  first [ eapply All_Remove_Lookup_inv with (a':=addr1) in H0'; eauto
+        | eapply All_Remove_Lookup_inv with (a':=addr2) in H0'; eauto ];
+  try (apply not_overlaps_sym; assumption).
+  - undecide; eapply not_overlaps_trans; eauto.
+  - apply not_overlaps_sym.
+    undecide; eapply not_overlaps_trans; eauto.
+  - eapply allocations_unique_r in H0; eauto.
+  - eapply allocations_unique_r in H0; eauto.
 Qed.
 
-Theorem find_partitions_a_singleton : forall r : Rep HeapSpec, fromADT _ r ->
+Corollary find_partitions_a_singleton : forall r : Rep HeapSpec, fromADT _ r ->
   forall addr base blk,
-    Find (fun a b => within a (memSize b) addr) base blk r
-      -> Partition (fun a b => within a (memSize b) addr) r
-           = (Single base blk, Remove base r).
+    Lookup base blk r
+      -> within base (memSize blk) addr
+      -> Same (Filter (fun a b => within a (memSize b) addr) r)
+              (Single base blk).
 Proof.
-  unfold Same; intros.
-  destruct H0.
+  intros.
   pose proof (allocations_no_overlap H _ H0).
-  pose proof (allocations_are_correct H).
   pose proof (allocations_unique H _ _ H0).
-  destruct (H3 (base, blk)); trivial;
-  simpl in *; clear H3 H5.
-  unfold Same_set, Included, Partition; f_equal.
-    unfold Single.
-    apply Compare.
-    split; intros.
-      unfold Included; intros.
-      simplify_ensembles; simpl in *.
-      destruct (N.eq_dec base n).
-        subst; specialize (H4 _ H7); subst.
-        constructor.
-      specialize (H2 _ _ H7 n0).
-      unfold within, overlaps in *; nomega.
-    simplify_ensembles.
-  unfold Remove.
-  apply Compare.
-  split; intros.
-    unfold Included; intros.
-    simplify_ensembles; simpl in *.
-    destruct (N.eq_dec base n).
-      subst; specialize (H4 _ H7); subst.
-      contradiction.
-    apply not_eq_sym.
-    exact n0.
-  simplify_ensembles.
-  unfold Ensembles.In in H5; simpl in H5.
-  apply not_eq_sym in H5.
-  specialize (H2 _ _ H3 H5).
-  unfold within, overlaps in *; nomega.
+  split; intros; inspect.
+    destruct (N.eq_dec base a); subst.
+      specialize (H3 _ H5); subst.
+      apply Lookup_Single; assumption.
+    specialize (H2 _ _ H5 n).
+    unfold overlaps, within in *; nomega.
+  apply Lookup_Filter; intuition.
 Qed.
 
 Corollary allocations_disjoint : forall r : Rep HeapSpec, fromADT _ r ->
   forall addr blk, Lookup addr blk r
     -> forall pos, within addr (memSize blk) pos
-    -> forall addr' blk',
-        Lookup addr' blk' r
-          -> addr <> addr'
-          -> ~ within addr' (memSize blk') pos.
+    -> forall addr' blk', Lookup addr' blk' r
+         -> addr <> addr'
+         -> ~ within addr' (memSize blk') pos.
 Proof.
   intros.
   pose proof (allocations_no_overlap H _ H0 _ H2 H3).
   unfold within, overlaps in *; nomega.
+Qed.
+
+Require Import Here.TupleEnsemblesFinite.
+
+Ltac finitary :=
+  repeat match goal with
+    | [ |- Finite _ Empty            ] => eapply Empty_Finite
+    | [ |- Finite _ (Single _ _)     ] => eapply Single_Finite
+    | [ |- Finite _ (Insert _ _ _ _) ] => eapply Insert_Finite
+    | [ |- Finite _ (Remove _ _)     ] => eapply Remove_Finite
+    | [ |- Finite _ (Setminus _)     ] => eapply Setminus_preserves_finite
+    | [ |- Finite _ (Update _ _ _)   ] => eapply Update_Finite
+    | [ |- Finite _ (Move _ _ _)     ] => eapply Move_Finite
+    | [ |- Finite _ (Filter _ _)     ] => eapply Filter_Finite
+    | [ |- Finite _ (Map _ _)        ] => eapply Map_Finite
+    | [ |- Finite _ (Modify _ _ _)   ] => eapply Modify_Finite
+    | [ |- Finite _ (Define _ _ _)   ] => eapply Define_Finite
+    | [ |- Finite _ (Overlay _ _ _)  ] => eapply Overlay_Finite
+    end; eauto.
+
+Theorem finite_heap : forall r : Rep HeapSpec, fromADT _ r -> Finite _ r.
+Proof. intros; ADT induction r; inspect; finitary. Qed.
+
+Theorem finite_blocks : forall r : Rep HeapSpec, fromADT _ r ->
+  All (fun _ blk => Finite _ (memData blk)) r.
+Proof.
+  unfold All; intros.
+  generalize dependent b.
+  generalize dependent a.
+  ADT induction r; inspect; finitary.
 Qed.
 
 End Heap.
@@ -547,7 +409,3 @@ Ltac tsubst :=
              ; memData := _ |} |- _ ] => inv H
     end;
   subst.
-
-Theorem neg_x_y_eq__x_y_eq : forall x y : bool,
-  negb x = negb y -> x = y.
-Proof. destruct 0, x; auto. Qed.
