FunMaps.v
@@ -1,5 +1,4 @@
 Require Import
-  Here.FunRelation
   Here.FMapExt
   Here.Nomega
   Coq.FSets.FMapList
