TupleEnsembles.v
@@ -1,0 +1,282 @@
+Require Import Coq.Sets.Ensembles.
+
+Generalizable All Variables.
+
+Section TupleEnsemble.
+
+Variables A B : Type.
+
+Definition Empty : Ensemble (A * B) := Empty_set _.
+
+Definition Single (a : A) (b : B) : Ensemble (A * B) :=
+  Singleton _ (a, b).
+
+Definition Lookup (a : A) (b : B) (r : Ensemble (A * B)) := In _ r (a, b).
+
+Definition Same (x y : Ensemble (A * B)) : Prop :=
+  forall a b, Lookup a b x <-> Lookup a b y.
+
+Definition Member (a : A) (r : Ensemble (A * B)) :=
+  exists b, Lookup a b r.
+
+Definition Insert (a : A) (b : B) (r : Ensemble (A * B))
+           (H : forall b' : B, ~ Lookup a b' r) : Ensemble (A * B) :=
+  Add _ r (a, b).
+
+Definition Remove (a : A) (r : Ensemble (A * B)) : Ensemble (A * B) :=
+  Setminus _ r (fun p => fst p = a).
+
+Require Import Coq.Program.Tactics.
+
+Program Definition Update (a : A) (b : B) (r : Ensemble (A * B)) :
+  Ensemble (A * B) :=
+  Insert a b (Remove a r) _.
+Obligation 1. firstorder. Qed.
+
+Definition Move (a a' : A) (r : Ensemble (A * B)) : Ensemble (A * B) :=
+  fun p => IF fst p = a'
+           then Lookup a (snd p) r
+           else Lookup (fst p) (snd p) (Remove a r).
+
+Definition Map (f : A -> B -> B) (r : Ensemble (A * B)) :
+  Ensemble (A * B) :=
+  fun p : A * B =>
+    exists b : B,
+      Lookup (fst p) b r /\
+      Lookup (fst p) (snd p) (Singleton _ (fst p, f (fst p) b)).
+
+Definition Filter (P : A -> B -> Prop) (r : Ensemble (A * B)) :
+  Ensemble (A * B) :=
+  fun p => Lookup (fst p) (snd p) r /\ P (fst p) (snd p).
+
+Definition Define (P : A -> Prop) (b : B) (r : Ensemble (A * B)) :
+  Ensemble (A * B) :=
+  fun p => IF P (fst p) then snd p = b else Lookup (fst p) (snd p) r.
+
+Definition Modify (a : A) (f : B -> B) (r : Ensemble (A * B)) :
+  Ensemble (A * B) :=
+  fun p => IF fst p = a
+           then exists b : B,
+                  Lookup (fst p) b r /\
+                  Lookup (fst p) (snd p) (Singleton _ (fst p, f b))
+           else Lookup (fst p) (snd p) r.
+
+Definition Overlay (P : A -> option A) (r' r : Ensemble (A * B)) :
+  Ensemble (A * B) :=
+  fun p =>
+    forall a,
+      IF P (fst p) = Some a
+      then Lookup a (snd p) r
+      else Lookup (fst p) (snd p) r'.
+
+Definition All (P : A -> B -> Prop) (r : Ensemble (A * B)) : Prop :=
+  forall a b, Lookup a b r -> P a b.
+
+Definition Any (P : A -> B -> Prop) (r : Ensemble (A * B)) : Prop :=
+  exists a b, Lookup a b r -> P a b.
+
+Lemma Lookup_Empty : forall a b, ~ Lookup a b Empty.
+Proof. firstorder. Qed.
+
+Lemma Lookup_Single : forall a b, Lookup a b (Single a b).
+Proof. firstorder. Qed.
+
+Lemma Lookup_Single_inv : forall a b c d,
+  Lookup a b (Single c d) -> a = c /\ b = d.
+Proof. split; inversion H; reflexivity. Qed.
+
+Lemma Lookup_Insert_inv : forall a b c d r H,
+  Lookup a b (Insert c d r H) -> (a = c /\ b = d) \/ Lookup a b r.
+Proof.
+  intros.
+  inversion H0; clear H0.
+    firstorder.
+  inversion H1; clear H1.
+  firstorder.
+Qed.
+
+Lemma Lookup_Remove : forall a b a' r,
+  Lookup a b r -> a <> a' -> Lookup a b (Remove a' r).
+Proof. firstorder. Qed.
+
+Lemma Lookup_Remove_ex_r : forall a b r,
+  Lookup a b r -> exists a', a <> a' -> Lookup a' b (Remove a r).
+Proof. firstorder. Qed.
+
+Lemma Lookup_Remove_inv : forall a b a' r,
+  Lookup a b (Remove a' r) -> a <> a' /\ Lookup a b r.
+Proof. firstorder. Qed.
+
+Lemma Lookup_Update_inv : forall a b a' b' r,
+  Lookup a b (Update a' b' r)
+    -> (a = a' /\ b = b') \/ (a <> a' /\ Lookup a b r).
+Proof.
+  intros.
+  inversion H; clear H.
+    firstorder.
+  inversion H0; clear H0.
+  firstorder.
+Qed.
+
+Lemma Lookup_Move_inv : forall a b a' a'' r,
+  Lookup a b (Move a' a'' r)
+    -> (a = a'' /\ Lookup a' b r) \/ (a <> a' /\ Lookup a b r).
+Proof. firstorder. Qed.
+
+Lemma Lookup_Map : forall a b f r,
+  Lookup a b r -> Lookup a (f a b) (Map f r).
+Proof. firstorder. Qed.
+
+Lemma Lookup_Map_inv : forall a b f r,
+  Lookup a b (Map f r) -> exists b', f a b' = b /\ Lookup a b' r.
+Proof.
+  intros.
+  inversion H; clear H.
+    firstorder.
+  inversion H0; clear H0.
+  firstorder.
+Qed.
+
+Lemma Lookup_Filter : forall a b P r,
+  Lookup a b r /\ P a b -> Lookup a b (Filter P r).
+Proof. firstorder. Qed.
+
+Lemma Lookup_Filter_inv : forall a b P r,
+  Lookup a b (Filter P r) -> P a b /\ Lookup a b r.
+Proof. firstorder. Qed.
+
+Lemma Lookup_Define_inv : forall a b c P r,
+  Lookup a b (Define P c r) -> (P a /\ b = c) \/ Lookup a b r.
+Proof. firstorder. Qed.
+
+Lemma Lookup_Modify_inv : forall a b a' f r,
+  Lookup a b (Modify a' f r)
+    -> (a = a' /\ exists b', f b' = b /\ Lookup a b' r)
+         \/ (a <> a' /\ Lookup a b r).
+Proof.
+  intros.
+  inversion H; clear H;
+  destruct H0.
+    destruct H0.
+    destruct H0.
+    inversion H1; simpl in *; subst.
+    left; split; trivial.
+    exists x.
+    split; trivial.
+  right; split; trivial.
+Qed.
+
+Lemma Lookup_Overlay_inv : forall a b P r' r,
+  Lookup a b (Overlay P r' r)
+    -> match P a with
+       | Some a' => Lookup a' b r
+       | None    => Lookup a b r'
+       end.
+Proof.
+  unfold Lookup, Overlay, Ensembles.In; simpl; intros.
+  destruct (P a).
+    destruct (H a0), H0.
+      exact H1.
+    tauto.
+  destruct (H a), H0.
+    discriminate.
+  exact H1.
+Qed.
+
+Lemma Lookup_Member : forall a b r,
+  Lookup a b r -> Member a r.
+Proof. firstorder. Qed.
+
+Lemma Member_Lookup_not : forall a r,
+  ~ Member a r -> forall b, ~ Lookup a b r.
+Proof. firstorder. Qed.
+
+Lemma All_Remove_inv : forall a P r,
+  All P (Remove a r) -> ~ Member a r -> All P r.
+Proof.
+  intros.
+  intros ???.
+  apply H.
+  apply Lookup_Remove.
+    assumption.
+  unfold not; intros.
+  subst.
+  unfold Member in H0.
+  Require Import Classical_Pred_Type.
+  apply not_ex_all_not with (n:=b) in H0.
+  contradiction.
+Qed.
+
+Lemma All_Remove_Lookup_inv : forall a P r,
+  All P (Remove a r) -> forall a' b', a <> a' -> Lookup a' b' r -> P a' b'.
+Proof. firstorder. Qed.
+
+End TupleEnsemble.
+
+Arguments Empty {_ _} _.
+Arguments Single : default implicits.
+Arguments Insert : default implicits.
+Arguments Remove : default implicits.
+Arguments Update : default implicits.
+Arguments Modify : default implicits.
+Arguments Move : default implicits.
+Arguments Filter : default implicits.
+Arguments Map : default implicits.
+Arguments All : default implicits.
+Arguments Any : default implicits.
+Arguments Define : default implicits.
+Arguments Overlay : default implicits.
+Arguments Lookup : default implicits.
+Arguments Same : default implicits.
+Arguments Member : default implicits.
+
+Arguments Lookup_Empty : default implicits.
+
+Ltac teardown :=
+  match goal with
+  | [ H : Lookup _ _ Empty           |- _ ] => contradiction (Lookup_Empty H)
+  | [ H : Lookup _ _ (Single _ _)    |- _ ] => apply Lookup_Single_inv in H
+  | [ H : Lookup _ _ (Insert _ _ _)  |- _ ] => apply Lookup_Insert_inv in H
+  | [ H : Lookup _ _ (Remove _ _)    |- _ ] => apply Lookup_Remove_inv in H
+  | [ H : Lookup _ _ (Update _ _ _)  |- _ ] => apply Lookup_Update_inv in H
+  | [ H : Lookup _ _ (Move _ _ _)    |- _ ] => apply Lookup_Move_inv in H
+  | [ H : Lookup _ _ (Map _ _)       |- _ ] => apply Lookup_Map_inv in H
+  | [ H : Lookup _ _ (Filter _ _)    |- _ ] => apply Lookup_Filter_inv in H
+  | [ H : Lookup _ _ (Define _ _ _)  |- _ ] => apply Lookup_Define_inv in H
+  | [ H : Lookup _ _ (Modify _ _ _)  |- _ ] => apply Lookup_Modify_inv in H
+  | [ H : Lookup _ _ (Overlay _ _ _) |- _ ] => apply Lookup_Overlay_inv in H
+
+  | [ H : Member _ Empty           |- _ ] => unfold Member in H
+  | [ H : Member _ (Single _ _)    |- _ ] => unfold Member in H
+  | [ H : Member _ (Insert _ _ _)  |- _ ] => unfold Member in H
+  | [ H : Member _ (Remove _ _)    |- _ ] => unfold Member in H
+  | [ H : Member _ (Update _ _ _)  |- _ ] => unfold Member in H
+  | [ H : Member _ (Move _ _ _)    |- _ ] => unfold Member in H
+  | [ H : Member _ (Map _ _)       |- _ ] => unfold Member in H
+  | [ H : Member _ (Filter _ _)    |- _ ] => unfold Member in H
+  | [ H : Member _ (Define _ _ _)  |- _ ] => unfold Member in H
+  | [ H : Member _ (Modify _ _ _)  |- _ ] => unfold Member in H
+  | [ H : Member _ (Overlay _ _ _) |- _ ] => unfold Member in H
+
+  | [ H : Lookup ?X ?Y ?R |- Member ?X ?R ] => exists Y; exact H
+
+  | [ H1 : All ?P ?R, H2 : Lookup ?X ?Y ?R |- _ ] =>
+    specialize (H1 _ _ H2); simpl in H1
+
+  | [ H : IF _ then _ else _ |- _ ] => destruct H
+  | [ H : _ /\ _             |- _ ] => destruct H
+  | [ H : _ * _              |- _ ] => destruct H
+  | [ H : exists _, _        |- _ ] => destruct H
+  | [ H : @sig _ _           |- _ ] => destruct H
+  | [ H : @sigT _ _          |- _ ] => destruct H
+  | [ H : bool               |- _ ] => destruct H
+  | [ H : option _           |- _ ] => destruct H
+  | [ H : _ \/ _             |- _ ] => destruct H
+
+  | [ H : forall x, Some ?X = Some x -> _  |- _ ] => specialize (H X eq_refl)
+  | [ H : forall x y, Some (?X, ?Y) = Some (x, y) -> _  |- _ ] =>
+    specialize (H X Y eq_refl)
+
+  | [ H1 : ?X = true, H2 : ?X = false |- _ ] => rewrite H1 in H2; discriminate
+
+  end; simpl in *; try tauto.
