TupleEnsemblesFinite.v
@@ -1,0 +1,80 @@
+Require Export
+  Here.TupleEnsembles
+  Coq.Sets.Finite_sets
+  Coq.Sets.Finite_sets_facts.
+
+Require Import
+  Coq.Program.Tactics.
+
+Generalizable All Variables.
+
+Section TupleEnsembleFinite.
+
+Variable A : Type.
+Variable B : Type.
+
+Lemma Empty_Finite : Finite _ (@Empty A B).
+Proof. constructor. Qed.
+
+Lemma Single_Finite : forall a b, Finite _ (@Single A B a b).
+Proof. intros; apply Singleton_is_finite. Qed.
+
+Lemma Insert_Finite : forall a b `(_ : Finite _ r) H, Finite _ (@Insert A B a b r H).
+Proof. intros; apply Add_preserves_Finite; assumption. Qed.
+
+Definition finite_ind := Generalized_induction_on_finite_sets.
+
+Lemma Setminus_preserves_finite {U} :
+  forall A:Ensemble U,
+    Finite U A -> forall X:Ensemble U, Finite U (Setminus U A X).
+Proof.
+  intros A' ? ?; apply Finite_downward_closed with A'; auto with sets.
+  intros ? H0; inversion H0; assumption.
+Qed.
+
+Lemma Conjunction_preserves_finite {U} :
+  forall A:Ensemble U,
+    Finite U A -> forall X:Ensemble U, Finite U (fun x : U => In U X x /\ In U A x).
+Proof.
+  intros A' H' X; apply Finite_downward_closed with A'; auto with sets.
+  intros ? H0; inversion H0; assumption.
+Qed.
+
+Lemma Remove_Finite : forall a `(_ : Finite _ r), Finite _ (@Remove A B a r).
+Proof.
+  unfold Remove; simpl; intros.
+  apply Setminus_preserves_finite; assumption.
+Qed.
+
+Lemma Update_Finite : forall a b `(_ : Finite _ r), Finite _ (@Update A B a b r).
+Proof.
+  unfold Remove; simpl; intros.
+  apply Add_preserves_Finite, Setminus_preserves_finite; assumption.
+Qed.
+
+Lemma Move_Finite : forall a a' `(_ : Finite _ r), Finite _ (@Move A B a a' r).
+Proof.
+Admitted.
+
+Lemma Filter_Finite : forall P `(_ : Finite _ r), Finite _ (@Filter A B P r).
+Proof.
+Admitted.
+
+Lemma Map_Finite : forall f `(_ : Finite _ r), Finite _ (@Map A B f r).
+Proof.
+Admitted.
+
+Lemma Modify_Finite : forall a f `(_ : Finite _ r), Finite _ (@Modify A B a f r).
+Proof.
+Admitted.
+
+Lemma Define_Finite : forall P b `(_ : Finite _ r), Finite _ (@Define A B P b r).
+Proof.
+Admitted.
+
+Lemma Overlay_Finite : forall P `(_ : Finite _ r) `(_ : Finite _ r'),
+  Finite _ (@Overlay A B P r r').
+Proof.
+Admitted.
+
+End TupleEnsembleFinite.
